modified:   cleanup.sh 	new file:   clojure/rabbitmq/clojure-1.6.jar 	new file:   clojure/rabbitmq/commons-cli-1.1.jar 	new file:   clojure/rabbitmq/commons-io-1.2.jar 	new file:   clojure/rabbitmq/compile.sh 	new file:   clojure/rabbitmq/hamcrest-core.jar 	new file:   clojure/rabbitmq/junit.jar 	new file:   clojure/rabbitmq/rabbitmq-client-tests.jar 	renamed:    clojure/rabbitmq-client.jar -> clojure/rabbitmq/rabbitmq-client.jar 	new file:   clojure/rabbitmq/run.sh 	new file:   clojure/rabbitmq/test_rabbitmq.clj 	modified:   coq/sort.v 	new file:   polyglot/Interpreter/interpreter.py 	modified:   polyglot/Interpreter/run.sh 	modified:   polyglot/Interpreter/search.sh

clojure/rabbitmq/test_rabbitmq.clj
@@ -1,0 +1,11 @@
+(ns test_rabbitmq
+  (:gen-class)
+  (:import (com.rabbitmq.client ConnectionFactory QueueingConsumer)))
+
+
+
+
+(defn -main []
+  (println "test_rabbitmq is running ...")
+
+)
