polyglot/Interpreter/interpreter.py
@@ -1,0 +1,136 @@
+# Interpreter Design Pattern
+
+# from the Gang of Four book:
+# "If a particular kind of problem occurs often enough, then it might be
+# worthwhile to express instances of the problem as sentences in a simple
+# language. Then you can build an interpreter that solves the problem by 
+# interpreting these sentences. For example, searching for strings that 
+# match a pattern is a common problem. Regular expressions are a standard 
+# language for specifying patterns of strings. Rather than building custom 
+# algorithms to match each pattern against strings, search algorithms could 
+# interpret a regular expression that specifies a set of strings to match."
+
+# Each regular expression r has an associated language L(r) (which is a set
+# of strings) defined by the recursion:
+#
+#  - r = Lit(s)        -> L(r) = {s}
+#  - r = And(r1, r2)   -> L(r) = L(r1).L(r2)     (see definition of '.')
+#  - r = Or(r1, r2)    -> L(r) = L(r1) U L(r2)
+#  - r = Many(r1)      -> L(r) = U_k L(r1)^k     (see definition of '.')
+#
+#  where given A,B sets of strings the product A.B is defined as the set of 
+#  strings A.B = { a ++ b | a in A, b in B }, and where it is understood that
+#  A^0 = {""} and A^1 = A. 
+#
+# Given a regular expression r and a string s, many reasonable questions 
+# can be asked in relation to r and s. When using the command 'grep', the
+# question being asked is whether there exist a substring s' of s which
+# belongs to the language of r. One of the first questions of interest is
+# of course whether s itself belongs to L(r).
+
+
+# There is no need to create static factory methods in python, as the
+# usual constructors have exactly the desired syntax
+class Exp():
+    # instance interface
+    def __str__(self):
+        raise NotImplementedError("Exp::__str__ is not implemented")
+    def interpret(self, input):
+        raise NotImplementedError("Exp::interpret is not implemented")
+    def recognize(self, input):
+        return input in self.interpret(input)
+
+
+class Lit(Exp):
+    def __init__(self, literal):
+        self._literal = literal
+    def __str__(self):
+        return self._literal
+    def interpret(self, input):
+        if input.startswith(self._literal): # _literal is a prefix of input
+            return [self._literal]
+        else:
+            return []
+
+class And(Exp):
+    def __init__(self, left, right):
+        self._left = left
+        self._right = right
+    def __str__(self):
+        return str(self._left) + str(self._right)
+    def interpret(self, input):
+        result = []
+        leftList = self._left.interpret(input)
+        for s1 in leftList:
+            remainder = input[len(s1):]
+            rightList = self._right.interpret(remainder)
+            for s2 in rightList:
+                result.append(s1 + s2)
+        return result
+
+class Or(Exp):
+    def __init__(self, left, right):
+        self._left = left
+        self._right = right
+    def __str__(self):
+        return "(" + str(self._left) + "|" + str(self._right) + ")"
+    def interpret(self, input):
+        return self._left.interpret(input) + self._right.interpret(input)
+
+
+class Many(Exp):
+    def __init__(self, regex):
+        self._regex = regex
+    def __str__(self):
+        return "(" + str(self._regex) + ")*"
+    def interpret(self, input):
+        result = [""]
+        leftList = self._regex.interpret(input)
+        for s1 in leftList:
+            if s1:  # s1 is not the empty string
+                remainder = input[len(s1):]
+                rightList = self.interpret(remainder)   # recursive call
+                for s2 in rightList:
+                    result.append(s1 + s2)
+        return result
+
+
+a = Lit("a")
+b = Lit("b")
+c = Lit("c")
+
+aa = And(a, Many(a))    # one or more 'a'
+bb = And(b, Many(b))    # one or more 'b'
+cc = And(c, Many(c))    # one or more 'c'
+
+regex = Many(And(Or(aa,bb),cc))
+string = "acbbccaaacccbbbbaaaaaccccc"
+
+print("regex = " + str(regex))
+print("string = \"" + string + "\"")
+print("The recognized prefixes are:")
+result = []
+for i in range(0,len(string)):
+    test = string[0:i]
+    if regex.recognize(test):
+        result.append("\"" + test + "\"")
+start = True
+print("[", end = "")
+for test in result:
+    if start:
+        start = False
+    else:
+        print(", ", end = "")
+    print(test, end = "")
+print("]")
+
+
+
+
+    
+
+
+
+
+
+
