clojure/rabbitmq/compile.sh
@@ -1,0 +1,7 @@
+#!/bin/sh
+RABBIT_JARS=
+for d in `dirname $0`/*.jar
+do
+    RABBIT_JARS="$d:$RABBIT_JARS"
+done
+clojurec -cp "$RABBIT_JARS" "$@"
